src/coq/Semantics/InfiniteToFinite.v
@@ -1,5 +1,8 @@
 From Coq Require Import
-     List Lia.
+     Relations
+     String
+     List
+     Lia.
 
 From Vellvm Require Import
      Semantics.InterpretationStack
@@ -224,9 +227,78 @@ Module InfiniteToFinite (IS1 : InterpreterStack) (IS2 : InterpreterStack) (AC1 :
   (* TODO: move this? *)
   Definition L5_convert_tree {T} (t : itree E1.L5 T) : itree E2.L5 T := interp L5_convert t.
 
-  Definition refine_oom {T} (sources : PropT E1.L5 T) (target : itree E2.L5 T) : Prop
-    := exists (source : itree E1.L5 T),
-      sources source ->
-      model_OOM_h (L5_convert_tree source) target.
+  (*
+  Definition refine_oom {T} (RR : relation T) (source : itree E1.L5 T) (target : itree E2.L5 T) : Prop
+    := model_OOM_h RR (L5_convert_tree source) target.
+   *)
+
+  From Coq Require Import RelationClasses.
+
+  Lemma refine_oom
+    : forall E F `{LLVMEvents.FailureE -< E +' F} T TT (HR: Reflexive TT)
+        (x : _ -> Prop)
+        (y : itree (E +' OOME +' F) T),
+      x y -> model_OOM TT x y.
+  Proof.
+    intros E F H T TT HR x y H0.
+    unfold model_OOM.
+    exists y. split. assumption.
+    unfold model_OOM_h.
+    apply interp_prop.
+    apply case_prop_handler_correct.
+    unfold handler_correct. intros. reflexivity.
+    apply case_prop_handler_correct.
+    apply UB_handler_correct.
+    unfold handler_correct. intros. reflexivity.
+    assumption. reflexivity.
+  Qed.
+
+  Lemma refine_oom_oom_void :
+    forall (source : itree E1.L5 void) (msg : string),
+      refine_oom eq source (trigger (ThrowOOM msg)).
+  Proof.
+    intros source msg.
+    cbn.
+    unfold refine_oom.
+
+    red.
+
+    Import InterpFacts.
+    Require Import PropT.
+
+    cbn.
+
+    rewrite interp_prop_trigger.
+
+
+  Qed.
+
+  Lemma refine_oom_oom :
+    forall {T : Type} (RR : relation T) (sources : PropT E1.L5 T) (t : itree E1.L5 T) (msg : string),
+      refine_oom RR sources (raise_oom msg).
+  Proof.
+    intros T RR sources t msg.
+    cbn.
+    unfold refine_oom.
+    exists t.
+    intros SOURCES.
+
+    red.
+
+    unfold L5_convert_tree.
+    Import InterpFacts.
+    unfold raiseOOM.
+    Require Import PropT.
+
+    Check (trigger (ThrowOOM msg)).
+    rewrite Eq.bind_trigger.
+    rewrite bind_trigger.
+    rewrite interp_prop _bind.
+    setoid_rewrite interp_interp.
+    epose proof interp_interp.
+
+    rewrite interp_ret.
+    exists t.
+  Qed.
 
 End InfiniteToFinite.
