src/coq/Theory/Refinement.v
@@ -30,6 +30,7 @@ From Coq Require Import Relations RelationClasses.
 Module Make (LP : LLVMParams) (LLVM : Lang LP).
   Import LP.
   Import LLVM.
+  Import LLVM.MEM.
 
   Module Conc := Serialization.Make ADDR IP SIZEOF Events PTOI PROV ITOP GEP Byte.
 
@@ -134,17 +135,17 @@ Module Make (LP : LLVMParams) (LLVM : Lang LP).
     := eutt refine_res2.
 
   (* For multiple CFG, after interpreting [LocalE] and [MemoryE] and [IntrinsicE] that are memory intrinsics *)
-  Definition refine_res3 : relation (memory_stack * (local_env * stack * (global_env * uvalue)))
+  Definition refine_res3 : relation (MemState * (local_env * stack * (global_env * uvalue)))
     := TT × refine_res2.
 
-  Definition refine_L3 : relation (itree L3 (memory_stack * (local_env * stack * (global_env * uvalue))))
+  Definition refine_L3 : relation (itree L3 (MemState * (local_env * stack * (global_env * uvalue))))
     := eutt refine_res3.
 
   (* Refinement for after interpreting pick. *)
-  Definition refine_L4 : relation ((itree L4 (memory_stack * (local_env * stack * (global_env * uvalue)))) -> Prop)
+  Definition refine_L4 : relation ((itree L4 (MemState * (local_env * stack * (global_env * uvalue)))) -> Prop)
     := fun ts ts' => forall t', ts' t' -> exists t, ts t /\ eutt refine_res3 t t'.
 
-  Definition refine_L5 : relation ((itree L5 (memory_stack * (local_env * stack * (global_env * uvalue)))) -> Prop)
+  Definition refine_L5 : relation ((itree L5 (MemState * (local_env * stack * (global_env * uvalue)))) -> Prop)
     := fun ts ts' => forall t', ts' t' -> exists t, ts t /\ eutt refine_res3 t t'.
 
 End Make.
